HLA dynamic semantics

mm0-lean/x86/hla.lean
@@ -83,37 +83,40 @@ inductive assemble_label (H : hla) : arg → qword → Prop
   c.2.1.nth n = some q →
   assemble_label (arg.llabel i n) q
 
-inductive assemble_imm_rm : arg → imm_rm → Prop
-| imm (q) : assemble_imm_rm (arg.imm q) (imm_rm.imm q)
-| reg (r) : assemble_imm_rm (arg.reg r) (imm_rm.rm (RM.reg r))
-| mem (si b q) : assemble_imm_rm
-  (arg.mem si b (bitvec.to_int q)) (imm_rm.rm (RM.mem si b q))
+def arg.imm_rm : arg → imm_rm → Prop
+| (arg.reg r) rm := imm_rm.rm (RM.reg r) = rm
+| (arg.mem ix b d) rm := imm_rm.rm (RM.mem ix b d) = rm
+| (arg.imm q) rm := imm_rm.imm q = rm
+| _ _ := false
 
-def assemble_imm (a : arg) (q : qword) : Prop :=
-assemble_imm_rm a (imm_rm.imm q)
+def arg.rm : arg → RM → Prop
+| (arg.reg r) rm := RM.reg r = rm
+| (arg.mem ix b d) rm := RM.mem ix b d = rm
+| _ _ := false
 
-def assemble_RM (a : arg) (rm : RM) : Prop :=
-assemble_imm_rm a (imm_rm.rm rm)
+theorem arg.rm_imm_rm {a rm} :
+  arg.rm a rm ↔ arg.imm_rm a (imm_rm.rm rm) :=
+by cases a; simp [arg.rm, arg.imm_rm]
 
 def assemble_ds (d s : arg) : dest_src → Prop
-| (dest_src.Rm_i rm q) := assemble_RM d rm ∧ assemble_imm s q
-| (dest_src.Rm_r rm r) := assemble_RM d rm ∧ assemble_RM s (RM.reg r)
-| (dest_src.R_rm r rm) := assemble_RM d (RM.reg r) ∧ assemble_RM s rm
+| (dest_src.Rm_i rm q) := arg.rm d rm ∧ s = arg.imm q
+| (dest_src.Rm_r rm r) := arg.rm d rm ∧ s = arg.reg r
+| (dest_src.R_rm r rm) := arg.rm d (RM.reg r) ∧ arg.rm s rm
 
 def code_pred := hla → list qword → qword → list byte → Prop
 
 def asm1.pred' : asm1 → ast → Prop
 | (asm1.unop op sz a) v := ∃ rm,
-  assemble_RM a rm ∧
+  a.rm rm ∧
   ast.unop op sz rm = v
 | (asm1.binop op sz d s) v := ∃ ds,
   assemble_ds d s ds ∧
   ast.binop op sz ds = v
 | (asm1.mul sz a) v := ∃ rm,
-  assemble_RM a rm ∧
+  a.rm rm ∧
   ast.mul sz rm = v
 | (asm1.div sz a) v := ∃ rm,
-  assemble_RM a rm ∧
+  a.rm rm ∧
   ast.div sz rm = v
 | (asm1.lea sz d s) v := ∃ ds,
   assemble_ds d s ds ∧
@@ -125,31 +128,162 @@ def asm1.pred' : asm1 → ast → Prop
   assemble_ds d s ds ∧
   ast.movzx sz ds sz2 = v
 | (asm1.xchg sz a r) v := ∃ rm,
-  assemble_RM a rm ∧
+  a.rm rm ∧
   ast.xchg sz rm r = v
 | (asm1.cmpxchg sz a r) v := ∃ rm,
-  assemble_RM a rm ∧
+  a.rm rm ∧
   ast.cmpxchg sz rm r = v
 | (asm1.xadd sz a r) v := ∃ rm,
-  assemble_RM a rm ∧
+  a.rm rm ∧
   ast.xadd sz rm r = v
 | (asm1.cmov c sz d s) v := ∃ ds,
   assemble_ds d s ds ∧
   ast.cmov c sz ds = v
 | (asm1.setcc c b a) v := ∃ rm,
-  assemble_RM a rm ∧
+  a.rm rm ∧
   ast.setcc c b rm = v
 | (asm1.push a) v := ∃ rm,
-  assemble_imm_rm a rm ∧
+  a.imm_rm rm ∧
   ast.push rm = v
 | (asm1.pop a) v := ∃ rm,
-  assemble_RM a rm ∧
+  a.rm rm ∧
   ast.pop rm = v
 | asm1.leave v := ast.leave = v
 | asm1.cmc v := ast.cmc = v
 | asm1.clc v := ast.clc = v
 | asm1.stc v := ast.stc = v
 | asm1.syscall v := ast.syscall = v
+
+theorem arg.imm_rm.determ {a rm1 rm2} : arg.imm_rm a rm1 → a.imm_rm rm2 → rm1 = rm2 :=
+by cases a; rintro ⟨⟩ ⟨⟩; refl
+
+theorem arg.rm.determ {a rm1 rm2} : arg.rm a rm1 → arg.rm a rm2 → rm1 = rm2 :=
+by cases a; rintro ⟨⟩ ⟨⟩; refl
+
+def arg.ea (k : config) (a : arg) (ea : EA) : Prop :=
+∃ rm, arg.imm_rm a rm ∧ imm_rm.ea k rm = ea
+
+theorem arg.ea.determ {k a ea1 ea2} : arg.ea k a ea1 → a.ea k ea2 → ea1 = ea2 :=
+by rintro ⟨_, h1, rfl⟩ ⟨_, h2, rfl⟩; cases h1.determ h2; refl
+
+theorem arg.imm_rm.ea {a rm k} (h : arg.imm_rm a rm) : arg.ea k a (rm.ea k) :=
+by cases a; cases h; exact ⟨_, rfl, rfl⟩
+
+theorem arg.rm.ea {a rm k} (h : arg.rm a rm) : arg.ea k a (rm.ea k) :=
+(arg.rm_imm_rm.1 h).ea
+
+theorem assemble_ds.src {d s ds k}
+  (h : assemble_ds d s ds) : arg.ea k s (ea_src k ds) :=
+begin
+  cases ds; cases h,
+  { subst s, exact ⟨_, rfl, rfl⟩ },
+  { subst s, refine ⟨_, rfl, rfl⟩ },
+  { exact h_right.ea },
+end
+
+theorem assemble_ds.dest {d s ds k}
+  (h : assemble_ds d s ds) : arg.ea k d (ea_dest k ds) :=
+by cases ds; cases h; exact h_left.ea
+
+def arg.read (k : config) (a : arg) (sz : wsize) (w : bitvec sz.to_nat) : Prop :=
+∃ ea, arg.ea k a ea ∧ ea.read k sz w
+
+def arg.readq (k : config) (a : arg) (sz : wsize) (q : qword) : Prop :=
+∃ ea, arg.ea k a ea ∧ ea.readq k sz q
+
+def arg.writeq (k : config) (a : arg) (sz : wsize) (q : qword) (k' : config) : Prop :=
+∃ ea, arg.ea k a ea ∧ ea.writeq k sz q k'
+
+def asm1.exec (k k' : config) : asm1 → Prop
+| (asm1.unop op sz rm) := ∃ ea w,
+  arg.ea k rm ea ∧ ea.readq k sz w ∧
+  write_unop sz w ea op k k'
+| (asm1.binop op sz d s) := ∃ ea d' s',
+  arg.ea k d ea ∧ ea.readq k sz d' ∧
+  s.readq k sz s' ∧
+  write_binop sz ea d' s' op k k'
+| (asm1.mul sz r) := ∃ eax src k2,
+  (EA.EA_r RAX).readq k sz eax ∧
+  r.readq k sz src ∧
+  match sz with
+  | (wsize.Sz8 _) :=
+    (EA.EA_r RAX).writeq k wsize.Sz16 (eax * src) k2
+  | _ := ∃ k1,
+    let hi := bitvec.of_nat sz.to_nat
+      ((eax.to_nat * src.to_nat).shiftl sz.to_nat) in
+    (EA.EA_r RAX).writeq k sz (eax * src) k1 ∧
+    (EA.EA_r RDX).writeq k1 sz (EXTZ hi) k2
+  end ∧
+  erase_flags k2 k'
+| (asm1.div sz r) := ∃ eax edx d k1 k2,
+  (EA.EA_r RAX).readq k sz eax ∧
+  (EA.EA_r RDX).readq k sz edx ∧
+  let n := edx.to_nat * (2 ^ sz.to_nat) + eax.to_nat in
+  r.readq k sz d ∧
+  let d := bitvec.to_nat d in
+  d ≠ 0 ∧ n / d < 2 ^ sz.to_nat ∧
+  (EA.EA_r RAX).writeq k sz (bitvec.of_nat _ (n / d)) k1 ∧
+  (EA.EA_r RDX).writeq k1 sz (bitvec.of_nat _ (n % d)) k2 ∧
+  erase_flags k2 k'
+| (asm1.lea sz d s) := ∃ sea,
+  arg.ea k s sea ∧
+  d.writeq k sz sea.addr k'
+| (asm1.movsx sz1 d s sz2) := ∃ w,
+  s.read k sz1 w ∧
+  d.writeq k sz2 (EXTZ (EXTS w : bitvec sz2.to_nat)) k'
+| (asm1.movzx sz1 d s sz2) := ∃ w,
+  s.read k sz1 w ∧
+  d.writeq k sz2 (EXTZ w) k'
+| (asm1.xchg sz r n) := ∃ dst val_src val_dst k1,
+  let src := EA.EA_r n in
+  r.ea k dst ∧
+  src.readq k sz val_src ∧
+  dst.readq k sz val_dst ∧
+  src.writeq k sz val_dst k1 ∧
+  dst.writeq k1 sz val_src k'
+| (asm1.cmpxchg sz r n) := ∃ dst val_dst val_acc,
+  let src := EA.EA_r n, acc := EA.EA_r RAX in
+  r.ea k dst ∧
+  dst.readq k sz val_dst ∧
+  acc.readq k sz val_acc ∧
+  (do
+    write_binop sz src val_acc val_dst binop.cmp,
+    if val_acc = val_dst then
+      src.read' sz >>= dst.write' sz
+    else acc.write' sz val_dst) k k'
+| (asm1.xadd sz r n) := ∃ dst val_src val_dst k1,
+  let src := EA.EA_r n in
+  r.ea k dst ∧
+  src.readq k sz val_src ∧
+  dst.readq k sz val_dst ∧
+  src.writeq k sz val_dst k1 ∧
+  write_binop sz dst val_src val_dst binop.add k1 k'
+| (asm1.cmov c sz d s) :=
+  cond (c.read k.flags)
+    (∃ w, s.readq k sz w ∧ d.writeq k sz w k')
+    (k = k')
+| (asm1.setcc c b r) :=
+  r.writeq k (wsize.Sz8 b) (EXTZ $ bitvec.singleton $ c.read k.flags) k'
+| (asm1.push i) := ∃ i',
+  arg.imm_rm i i' ∧ push i' k k'
+| (asm1.pop r) := ∃ r',
+  arg.rm r r' ∧ pop r' k k'
+| asm1.leave :=
+  pop (RM.reg RBP) (k.set_reg RSP (k.regs RBP)) k'
+| asm1.clc := k' = {flags := {CF := ff, ..k.flags}, ..k}
+| asm1.cmc := k' = {flags := {CF := bnot k.flags.CF, ..k.flags}, ..k}
+| asm1.stc := k' = {flags := {CF := tt, ..k.flags}, ..k}
+| asm1.syscall := false
+
+def noIO_rel (P : config → config → Prop) : kcfg → kcfg → Prop
+| ⟨i, o, k⟩ ⟨i', o', k'⟩ := i = i' ∧ o = o' ∧ P k k'
+
+def asm1.kexec : kcfg → kcfg → asm1 → Prop
+| ⟨i, o, k⟩ ⟨i', o', k'⟩ asm1.syscall := ∃ k1 k2 ret,
+  config.isIO k k1 ∧
+  exec_io i o k1 (k1.regs RAX) i' o' k2 ret →
+  k' = k2.set_reg RAX ret
+| ⟨i, o, k⟩ ⟨i', o', k'⟩ a := i = i' ∧ o = o' ∧ a.exec k k'
 
 def asm1.pred (a : asm1) : code_pred :=
 λ _ _ _ v, ∃ a', a.pred' a' ∧ decode a' v
@@ -164,12 +298,27 @@ def terminator.pred : terminator → code_pred
   labs.nth e = some (q + v.length)
 | (terminator.call f e) H labs rip v := ∃ q,
   assemble_label H (arg.label f) q ∧
-  decode (ast.call (imm_rm.imm q)) v ∧
+  decode (ast.call (imm_rm.imm (q - rip))) v ∧
   labs.nth e = some (q + v.length)
 | terminator.syscall_exit H labs rip v :=
   decode ast.syscall v -- this is ensured to be 'exit' syscall elsewhere
 | terminator.ret H labs rip v :=
   decode (ast.ret 0) v
+
+def terminator.exec (H : hla) (labs : list qword) (k : config) (k' : config ⊕ qword) : terminator → Prop
+| (terminator.jump a) := ∃ q,
+  assemble_label H a q ∧
+  k' = sum.inl {rip := q, ..k}
+| (terminator.jcc c i e) := ∃ q,
+  labs.nth (cond (c.read k.flags) i e) = some q ∧
+  k' = sum.inl {rip := q, ..k}
+| (terminator.call f e) := ∃ k1 w q,
+  labs.nth e = some w ∧
+  push_aux w k k1 ∧
+  assemble_label H (arg.label f) q ∧
+  k' = sum.inl {rip := q, ..k}
+| terminator.syscall_exit := ∃ q, config.exit k q ∧ k' = sum.inr q
+| terminator.ret := ∃ k1, pop_rip k k1 ∧ k' = sum.inl k1
 
 def code_pred.cons (c1 c2 : code_pred) : code_pred :=
 λ H labs rip v,
@@ -180,6 +329,15 @@ def code_pred.cons (c1 c2 : code_pred) : code_pred :=
 def bblock.pred : bblock → code_pred
 | (bblock.cons a b) := a.pred.cons b.pred
 | (bblock.term t) := t.pred
+
+structure kexit := (input output : list byte) (exit_code : qword)
+
+def bblock.kexec (H : hla) (labs : list qword) : bblock → kcfg → kcfg ⊕ kexit → Prop
+| (bblock.cons a b) k k' := ∃ k1, a.kexec k k1 ∧ b.kexec k1 k'
+| (bblock.term t) ⟨i, o, k⟩ (sum.inl ⟨i', o', k'⟩) :=
+   i = i' ∧ o = o' ∧ t.exec H labs k (sum.inl k')
+| (bblock.term t) ⟨i, o, k⟩ (sum.inr ⟨i', o', c⟩) :=
+   i = i' ∧ o = o' ∧ t.exec H labs k (sum.inr c)
 
 def code_pred.ok (C : code_pred) (H : hla) (k : config) (labs : list qword) :=
 ∃ v, C H labs k.rip v ∧ k.mem.read' (perm.R + perm.X) k.rip v
@@ -197,6 +355,140 @@ inductive bblocks.pred' (H : hla) (labs : list qword) :
 def hla.blocks (H : hla) (l : list (list bblock)) : Prop :=
 ∀ i q n ll v, H.code.nth i = some ((q, n), (ll, v)) →
   ∃ bs, l.nth i = some bs ∧ bblocks.pred' H ll bs ll q v
+
+theorem asm1.exec_ok {a a'} (ha : asm1.pred' a a') {k k'} :
+  execute a' k k' ↔ a.exec k k' :=
+begin
+  change (execute a' k).P () k' ↔ _,
+  cases a,
+  case hla.asm1.unop : op sz a {
+    rcases ha with ⟨rm, h1, rfl⟩,
+    split,
+    { rintro ⟨_, _, ⟨⟩, q, _, ⟨h2, rfl⟩, h3⟩,
+      exact ⟨_, _, h1.ea, h2, h3⟩ },
+    { rintro ⟨ea, q, ⟨rm', h1', rfl⟩, h2, h3⟩,
+      cases (arg.rm_imm_rm.1 h1).determ h1',
+      exact ⟨_, _, ⟨_⟩, q, _, ⟨h2, rfl⟩, h3⟩ } },
+  case hla.asm1.binop : op sz d s {
+    rcases ha with ⟨ds, h1, rfl⟩,
+    split,
+    { rintro ⟨⟨ea, d', s'⟩, _, ⟨⟨d, s, h2, h3⟩, rfl⟩, h4⟩,
+      exact ⟨_, _, _, h1.dest, h2, ⟨_, h1.src, h3⟩, h4⟩ },
+    { rintro ⟨_, d', s', hd, h3, ⟨s'', hs, _, h4, rfl⟩, h5⟩,
+      cases h1.dest.determ hd,
+      cases h1.src.determ hs,
+      exact ⟨⟨_, _, _⟩, _, ⟨⟨_, _, h3, _, h4, rfl⟩, rfl⟩, h5⟩ } },
+  case hla.asm1.mul : sz a {
+    rcases ha with ⟨rm, h1, rfl⟩,
+    split,
+    { rintro ⟨q, _, ⟨h2, rfl⟩, _, _, ⟨⟩,
+        q2, _, ⟨h3, rfl⟩, ⟨⟩, k1, h4, h5⟩,
+      refine ⟨_, _, _, h2, ⟨_, h1.ea, h3⟩, _, h5⟩,
+      cases sz, exact h4,
+      all_goals { rcases h4 with ⟨⟨⟩, k, h1, h2⟩, exact ⟨_, h1, h2⟩ } },
+    { rintro ⟨q, w, k1, h2, ⟨_, h1', h3⟩, h4, h5⟩,
+      cases h1.ea.determ h1',
+      refine ⟨_, _, ⟨h2, rfl⟩, _, _, ⟨_⟩, _, _, ⟨h3, rfl⟩, ⟨⟩, _, _, h5⟩,
+      cases sz, exact h4,
+      all_goals { rcases h4 with ⟨_, h1, h2⟩, exact ⟨⟨⟩, _, h1, h2⟩ } } },
+  case hla.asm1.div : sz a {
+    rcases ha with ⟨rm, h1, rfl⟩,
+    split,
+    { rintro ⟨eax, _, ⟨h2, rfl⟩, edx, _, ⟨h3, rfl⟩, _, _, ⟨⟩, _, _,
+        ⟨d, _, ⟨h4, rfl⟩⟩, ⟨⟩, _, ⟨⟨h5, h6⟩, rfl⟩, ⟨⟩, _, h7, ⟨⟩, _, h8⟩,
+      exact ⟨_, _, _, _, _, h2, h3, ⟨_, h1.ea, h4⟩, h5, h6, h7, h8⟩ },
+    { rintro ⟨_, _, _, _, _, h2, h3, ⟨_, h1', h4⟩, h5, h6, h7, h8⟩,
+      cases h1.ea.determ h1',
+      exact ⟨_, _, ⟨h2, rfl⟩, _, _, ⟨h3, rfl⟩, _, _, ⟨_⟩, _, _,
+        ⟨_, _, _, ⟨h4, rfl⟩⟩, ⟨⟩, _, ⟨⟨h5, h6⟩, rfl⟩, ⟨⟩, _, h7, ⟨⟩, _, h8⟩ } },
+  case hla.asm1.lea : sz d s {
+    rcases ha with ⟨ds, h1, rfl⟩,
+    split,
+    { rintro ⟨_, _, ⟨⟩, h2⟩,
+      exact ⟨_, h1.src, _, h1.dest, h2⟩ },
+    { rintro ⟨_, hs, _, hd, h2⟩,
+      cases h1.dest.determ hd,
+      cases h1.src.determ hs,
+      exact ⟨_, _, ⟨_⟩, h2⟩ } },
+  iterate 2 {
+    rcases ha with ⟨ds, h1, rfl⟩,
+    split,
+    { rintro ⟨_, _, ⟨h2, rfl⟩, _, _, ⟨⟩, h3⟩,
+      exact ⟨_, ⟨_, h1.src, h2⟩, _, h1.dest, h3⟩ },
+    { rintro ⟨_, ⟨_, hs, h2⟩, _, hd, h3⟩,
+      cases h1.dest.determ hd,
+      cases h1.src.determ hs,
+      exact ⟨_, _, ⟨h2, rfl⟩, _, _, ⟨_⟩, h3⟩ } },
+  case hla.asm1.xchg : sz a r {
+    rcases ha with ⟨rm, h1, rfl⟩,
+    split,
+    { rintro ⟨_, _, ⟨⟩, _, _, ⟨h2, rfl⟩, _, _, ⟨h3, rfl⟩, ⟨⟩, _, h4⟩,
+      exact ⟨_, _, _, _, h1.ea, h2, h3, h4⟩ },
+    { rintro ⟨_, _, _, _, h1', h2, h3, h4⟩,
+      cases h1.ea.determ h1',
+      exact ⟨_, _, ⟨_⟩, _, _, ⟨h2, rfl⟩, _, _, ⟨h3, rfl⟩, ⟨⟩, _, h4⟩ } },
+  case hla.asm1.cmpxchg : sz a r {
+    rcases ha with ⟨rm, h1, rfl⟩,
+    split,
+    { rintro ⟨_, _, ⟨⟩, _, _, ⟨h2, rfl⟩, _, _, ⟨h3, rfl⟩, h4⟩,
+      exact ⟨_, _, _, h1.ea, h2, h3, h4⟩ },
+    { rintro ⟨_, _, _, h1', h2, h3, h4⟩,
+      cases h1.ea.determ h1',
+      exact ⟨_, _, ⟨_⟩, _, _, ⟨h2, rfl⟩, _, _, ⟨h3, rfl⟩, h4⟩ } },
+  case hla.asm1.xadd : sz a r {
+    rcases ha with ⟨rm, h1, rfl⟩,
+    split,
+    { rintro ⟨_, _, ⟨⟩, _, _, ⟨h2, rfl⟩, _, _, ⟨h3, rfl⟩, ⟨⟩, _, h4⟩,
+      exact ⟨_, _, _, _, h1.ea, h2, h3, h4⟩ },
+    { rintro ⟨_, _, _, _, h1', h2, h3, h4⟩,
+      cases h1.ea.determ h1',
+      exact ⟨_, _, ⟨_⟩, _, _, ⟨h2, rfl⟩, _, _, ⟨h3, rfl⟩, ⟨⟩, _, h4⟩, } },
+  case hla.asm1.cmov : c sz d s {
+    rcases ha with ⟨ds, h1, rfl⟩,
+    change _ ↔ cond _ _ _,
+    split,
+    { rintro ⟨_, _, ⟨⟩, h2⟩, dsimp only at h2,
+      revert h2, cases c.read k.flags,
+      { rintro ⟨⟩, exact rfl },
+      { rintro ⟨_, _, ⟨h3, rfl⟩, h4⟩,
+        exact ⟨_, ⟨_, h1.src, h3⟩, _, h1.dest, h4⟩ } },
+    { intro h2, refine ⟨_, _, ⟨_⟩, _⟩, dsimp only,
+      revert h2, cases c.read k.flags,
+      { rintro ⟨⟩, exact ⟨_, _⟩ },
+      { rintro ⟨_, ⟨_, hs, h3⟩, _, hd, h4⟩,
+        cases h1.dest.determ hd,
+        cases h1.src.determ hs,
+        exact ⟨_, _, ⟨h3, rfl⟩, h4⟩ } } },
+  case hla.asm1.setcc : c b a {
+    rcases ha with ⟨rm, h1, rfl⟩,
+    split,
+    { rintro ⟨_, _, ⟨⟩, h2⟩,
+      exact ⟨_, h1.ea, h2⟩ },
+    { rintro ⟨_, h1', h2⟩,
+      cases h1.ea.determ h1',
+      exact ⟨_, _, ⟨_⟩, h2⟩ } },
+  iterate 2 {
+    rcases ha with ⟨rm, h1, rfl⟩,
+    split,
+    { exact λ h2, ⟨_, h1, h2⟩ },
+    { rintro ⟨_, h1', h2⟩,
+      cases h1.determ h1',
+      exact h2 } },
+  case hla.asm1.leave {
+    cases ha, split,
+    { rintro ⟨_, _, ⟨_, _, ⟨h2, rfl⟩, h3⟩, h4⟩,
+      cases EA.readq_reg_64.1 h2,
+      cases EA.writeq_reg_64.1 h3,
+      exact h4 },
+    { rintro h4,
+      exact ⟨⟨⟩, _, ⟨_, _,
+        ⟨EA.readq_reg_64.2 rfl, rfl⟩, EA.writeq_reg_64.2 rfl⟩, h4⟩ } },
+  iterate 3 {
+    cases ha, split,
+    { rintro ⟨⟩, constructor },
+    { rintro ⟨⟩, constructor } },
+  case hla.asm1.syscall { cases ha, split; rintro ⟨⟨⟩⟩ },
+end
 
 theorem code_pred.cons_ok {a b H k labs}
   (h : (code_pred.cons a b).ok H k labs) : a.ok H k labs := sorry
